WIP

src/example/FairLock.v
@@ -2,7 +2,9 @@ From sflib Require Import sflib.
 From Paco Require Import paco.
 Require Import Coq.Classes.RelationClasses Lia Program.
 Unset Universe Checking.
-From Fairness Require Export ITreeLib WFLib FairBeh NatStructs Mod pind Axioms OpenMod SCM Red IRed Wrapper.
+From Fairness Require Export
+     ITreeLib WFLib FairBeh NatStructs Mod pind Axioms
+     OpenMod SCM Red IRed Wrapper.
 From PromisingSEQ Require Import TView.
 From Ordinal Require Export ClassicalHessenberg.
 
@@ -51,6 +53,55 @@ Module AbsLock.
                      ("unlock", Mod.wrap_fun unlock_fun)]).
 
 End AbsLock.
+
+Module AbsLockW.
+
+  Definition lock_fun
+    : ktree (((@eventE thread_id) +' cE) +' (sE ((option TView.t) * NatMap.t unit)%type))
+            TView.t TView.t :=
+    fun tvw =>
+      _ <- trigger Yield;;
+      tid <- trigger (GetTid);;
+      '(own, ts) <- trigger (@Get _);;
+      let ts := NatMap.add tid tt ts in
+      _ <- trigger (Put (own, ts));;
+      `tvw_lock: TView.t <- (ITree.iter
+                              (fun (_: unit) =>
+                                 _ <- trigger Yield;;
+                                 '(own, ts) <- trigger (@Get _);;
+                                 match own with
+                                 | None => Ret (inl tt)
+                                 | Some tvw_lock => Ret (inr tvw_lock)
+                                 end)
+                              tt);;
+      '(_, ts) <- trigger (@Get _);;
+      let ts := NatMap.remove tid ts in
+      _ <- trigger (Put (None, ts));;
+      _ <- trigger (Fair (fun i => if tid_dec i tid then Flag.success
+                               else if (NatMapP.F.In_dec ts i) then Flag.fail
+                                    else Flag.emp));;
+      _ <- trigger Yield;;
+      Ret (TView.join tvw tvw_lock).
+
+  Definition unlock_fun
+    : ktree (((@eventE thread_id) +' cE) +' (sE ((option TView.t) * NatMap.t unit)%type))
+            TView.t TView.t :=
+    fun tvw =>
+      _ <- trigger Yield;;
+      '(own, ts) <- trigger (@Get _);;
+      match own with
+      | None => _ <- trigger (Put (Some tvw, ts));; _ <- trigger Yield;; Ret tvw
+      | Some _ => UB
+      end.
+
+  Definition mod: Mod.t :=
+    Mod.mk
+      (Some TView.bot, NatMap.empty unit)
+      (Mod.get_funs [("lock", Mod.wrap_fun lock_fun);
+                     ("unlock", Mod.wrap_fun unlock_fun)]).
+
+End AbsLockW.
+
 
 Module FairLock.
   Definition lock_fun: WMod.function bool unit void :=
