src/example/WMM.v
@@ -122,3 +122,61 @@ Module WMem.
                      ("faa", Mod.wrap_fun faa_fun)
       ]).
 End WMem.
+
+From Fairness Require Import PCM IProp IPM StateRA MonotonePCM.
+
+Section MEMRA.
+  Definition wmemRA: URA.t.
+  Admitted.
+
+  Context `{WMEMRA: @GRA.inG wmemRA Σ}.
+
+  Definition wmemory_black (m: WMem.t): iProp.
+  Admitted.
+
+  Definition wpoints_to (l: Loc.t) (v: Const.t) (vw: TView.t): iProp.
+  Admitted.
+
+  Lemma wpoints_to_view_mon l v vw0 vw1
+        (LE: TView.le vw0 vw1)
+    :
+    (wpoints_to l v vw0)
+      ⊢
+      (wpoints_to l v vw1).
+  Proof.
+  Admitted.
+
+  Lemma wmemory_ra_load
+        m l v vw0 vw1
+        ord lc1 to released
+        (READ: Local.read_step (Local.mk vw0 Memory.bot) m.(WMem.memory) l to v released ord lc1)
+        (VIEW: vw1 = lc1.(Local.tview))
+        (ORD: ord = Ordering.plain)
+    :
+    (wmemory_black m)
+      -∗
+      (wpoints_to l v vw0)
+      -∗
+      ((wmemory_black m) ∗ (⌜TView.le vw0 vw1⌝) ∗ #=>(wpoints_to l v vw1)).
+  Proof.
+  Admitted.
+
+  Lemma wmemory_ra_store
+        m0 l v0 vw0 m1 v1 vw1
+        lc1 to sc1 mem1 ord from released kind
+        (WRITE: Local.write_step (Local.mk vw0 Memory.bot) m0.(WMem.sc) m0.(WMem.memory) l from to v1 None released ord lc1 sc1 mem1 kind)
+        (VIEW: vw1 = lc1.(Local.tview))
+        (MEM: m1 = WMem.mk mem1 sc1)
+        (ORD: ord = Ordering.plain)
+    :
+    (wmemory_black m0)
+      -∗
+      (wpoints_to l v0 vw0)
+      -∗
+      ((⌜TView.le vw0 vw1⌝) ∗ #=>((wmemory_black m1) ∗ (wpoints_to l v1 vw1))).
+  Proof.
+  Admitted.
+
+End MEMRA.
+
+Global Opaque wpoints_to wmemory_black.
